high/Veritas.Record.fsti
@@ -54,3 +54,21 @@ let init_value (k:key): v:value{is_value_of k v} =
 let to_merkle_value (v:value{MVal? v}) = MVal?.v v
 
 let to_data_value (v:value{DVal? v}) = DVal?.v v
+
+let mv_points_to_none (v: merkle_value) (d:bin_tree_dir): bool = 
+  desc_hash_dir v d = Empty
+
+let mv_points_to_some (v:merkle_value) (d:bin_tree_dir): bool = 
+  Desc? (desc_hash_dir v d) 
+
+let mv_pointed_key (v:merkle_value) (d:bin_tree_dir{mv_points_to_some v d}): key = 
+  Desc?.k (desc_hash_dir v d)
+
+let mv_pointed_hash (v:merkle_value) (d:bin_tree_dir{mv_points_to_some v d}): hash_value = 
+  Desc?.h (desc_hash_dir v d)
+
+let mv_points_to (v:merkle_value) (d:bin_tree_dir) (k:key): bool = 
+  mv_points_to_some v d && mv_pointed_key v d = k
+
+let mv_evicted_to_blum (v:merkle_value) (d:bin_tree_dir {mv_points_to_some v d}): bool =
+  Desc?.b (desc_hash_dir v d)
