intermediate/Veritas.Intermediate.Logs.fsti
@@ -1,0 +1,183 @@
+module Veritas.Intermediate.Logs
+
+open FStar.Seq
+open Veritas.BinTree
+open Veritas.Key
+open Veritas.MultiSetHashDomain
+open Veritas.Record
+open Veritas.SeqAux
+open Veritas.State
+
+open Veritas.Intermediate.VerifierConfig
+open Veritas.Intermediate.SlotKeyRel
+
+module Spec = Veritas.Verifier
+
+(* Definitions of different styles of verifier logs.
+   - logK : contains only key references (defined in Veritas.Verifier)
+   - logS: contains slot references
+   - logL: contains slot references & low-level data structures (TODO) *)
+
+let thread_id = Spec.thread_id
+
+let logK_entry = Spec.vlog_entry
+let logK = Spec.vlog
+
+type logS_entry (vcfg:verifier_config) =
+  | Get_S: s:slot_id vcfg -> k:data_key -> v:data_value -> logS_entry vcfg
+  | Put_S: s:slot_id vcfg -> k:data_key -> v:data_value -> logS_entry vcfg
+  | AddM_S: s:slot_id vcfg -> r:record -> s':slot_id vcfg -> logS_entry vcfg
+  | EvictM_S: s:slot_id vcfg -> s':slot_id vcfg -> logS_entry vcfg
+  | AddB_S: s:slot_id vcfg -> r:record -> t:timestamp -> j:thread_id -> logS_entry vcfg
+  | EvictB_S: s:slot_id vcfg -> t:timestamp -> logS_entry vcfg
+  | EvictBM_S: s:slot_id vcfg -> s':slot_id vcfg -> t:timestamp -> logS_entry vcfg
+             
+let logS vcfg = Seq.seq (logS_entry vcfg)
+
+let is_state_op #vcfg (e: logS_entry vcfg): bool =
+  match e with
+  | Get_S _ _ _ | Put_S _ _ _ -> true
+  | _ -> false
+
+let to_state_op #vcfg (e:logS_entry vcfg {is_state_op e}): state_op =
+  match e with
+  | Get_S _ k v -> Get k v
+  | Put_S _ k v -> Put k v
+
+let to_state_op_logS #vcfg (l: logS vcfg) =
+  map to_state_op (filter_refine is_state_op l)
+
+(* 
+ * Given a slot -> key mapping, we define a boolean whether a log entry is valid.
+ * This definition checks if the slots are used correctly:
+ * (a) We add to a slot only if it is free
+ * (b) We evict from a slot only if it is associated with a key
+ * (c) We reference a slot in Get/Put and as an ancestor in Add/Evict only if it is associated with a key
+ *) 
+let valid_logS_entry #vcfg (ssm: slot_state_map vcfg) (e: logS_entry vcfg): bool = 
+  match e with
+  | Get_S s k _
+  | Put_S s k _ -> 
+    is_assoc_with ssm s k
+  | AddM_S s (k,_) s' -> 
+    is_free ssm s && is_assoc ssm s'
+  | AddB_S s (k,_) _ _ ->
+    is_free ssm s
+  | EvictM_S s s' ->
+    is_assoc ssm s && is_assoc ssm s'
+  | EvictB_S s _ ->
+    is_assoc ssm s
+  | EvictBM_S s s' _ ->
+    is_assoc ssm s && is_assoc ssm s'
+
+let to_logK_entry #vcfg (ssm: slot_state_map vcfg) (e: logS_entry vcfg{valid_logS_entry ssm e}): logK_entry = 
+  match e with
+  | Get_S s k v -> Spec.Get k v
+  | Put_S s k v -> Spec.Put k v
+  | AddM_S s r s' -> Spec.AddM r (assoc_key ssm s')    
+  | AddB_S s r t j -> Spec.AddB r t j    
+  | EvictM_S s s' -> Spec.EvictM (assoc_key ssm s) (assoc_key ssm s')
+  | EvictB_S s t -> Spec.EvictB (assoc_key ssm s) t
+  | EvictBM_S s s' t -> Spec.EvictBM (assoc_key ssm s) (assoc_key ssm s') t
+  
+(* 
+ * define a state machine over slot_states; to allow for "failures" where the log 
+ * uses slot states in an inconsistent manner (e.g., evict a slot without adding to it) 
+ * we make the transition function return option slot_state, with None being failure. 
+ *)
+let slot_state_trans #vcfg (e:logS_entry vcfg) (s:slot_id vcfg) (sst: slot_state): option slot_state = 
+  match e with
+  | Get_S s1 k1 _
+  | Put_S s1 k1 _ -> 
+    if s = s1 then 
+      if Assoc? sst && Assoc?.k sst = k1 then Some sst
+      else None
+    else Some sst
+  | AddM_S s1 (k1,_) s2 -> 
+    if s = s1 then 
+      if Free? sst then Some (Assoc k1)
+      else Some sst
+    else if s = s2 then
+      if Assoc? sst then Some sst
+      else None
+    else Some sst
+  | AddB_S s1 (k1,_) _ _ ->
+    if s = s1 then
+      if Free? sst then Some (Assoc k1)
+      else None
+    else Some sst
+  | EvictM_S s1 s2 ->
+    if s = s1 then
+      if Assoc? sst then Some Free
+      else None
+    else if s = s2 then
+      if Assoc? sst then Some sst
+      else None
+    else Some sst
+  | EvictB_S s1 _ ->
+    if s = s1 then
+      if Assoc? sst then Some Free
+      else None
+    else Some sst
+  | EvictBM_S s1 s2 _ ->
+    if s = s1 then
+      if Assoc? sst then Some Free
+      else None
+    else if s = s2 then
+      if Assoc? sst then Some sst
+      else None
+    else Some sst
+
+let rec slot_state_trans_closure #vcfg (s:slot_id vcfg) (l:logS vcfg) (sst_init: slot_state)
+  : Tot (option slot_state) (decreases (length l)) =     
+  let n = length l in
+  if n = 0 then Some (sst_init)
+  else 
+    let l' = hprefix l in
+    let e = telem l in
+    let osst' = slot_state_trans_closure s l' sst_init in
+    if None? osst' then None
+    else 
+    slot_state_trans e s (Some?.v osst')
+
+(* 
+ * a consistent log that uses/references slots in a correct way:
+ *  (a) Add associates a slot with a key
+ *  (b) a slot is evicted if it is currently associated with a key
+ *  (c) a slot is referenced in get/put and add/evict (as an ancestor) only if it is currently associated with a keys
+ *  (d) An add is over a currently free slot 
+ *  (e) the definition uses an initial slot -> state mapping; we do not start with a mapping where all slots are free since 
+ *      we want to start verifier thread 0 with Root in slot 0
+ *) 
+let consistent_log #vcfg (init_map: slot_state_map vcfg) (l:logS vcfg) = 
+  forall (s:slot_id vcfg). {:pattern slot_state_trans_closure s l (init_map s)}  slot_state_trans_closure s l (init_map s) <> None
+
+(* a consistent log maps an initial slot_state_map to another slot_state_map *)
+let to_slot_state_map #vcfg (init_map: slot_state_map vcfg) (l:logS vcfg{consistent_log init_map l}): slot_state_map _ = 
+  fun s -> Some?.v (slot_state_trans_closure s l (init_map s))
+
+(* prefix of a consistent log is consistent *)
+val lemma_consistent_log_prefix_consistent (#vcfg:_) (init_map: slot_state_map vcfg) (l:logS vcfg) (i:nat{i <= length l}):
+  Lemma (requires (consistent_log init_map l))
+        (ensures (consistent_log init_map (prefix l i)))
+
+(* consistent logs can be mapped to spec-level log by replacing all slot references to the assoc'ed keys *)
+val to_logk (#vcfg:_) (init_map: slot_state_map vcfg) (l:logS vcfg{consistent_log init_map l}): logK
+
+val lemma_to_logk_length (#vcfg:_) (init_map: slot_state_map vcfg) (l:logS vcfg{consistent_log init_map l}):
+  Lemma (ensures (length (to_logk init_map l) = length l))
+        [SMTPat (to_logk init_map l)]
+
+val lemma_all_entries_valid (#vcfg:_) (init_map: slot_state_map vcfg) (l:logS vcfg{consistent_log init_map l}) (i:seq_index l):
+  Lemma (ensures (let l' = prefix l i in
+                  lemma_consistent_log_prefix_consistent init_map l i;
+                  let ssm' = to_slot_state_map init_map l' in
+                  valid_logS_entry ssm' (index l i)))
+
+val lemma_to_logk_index (#vcfg:_) (init_map: slot_state_map vcfg) (l:logS _{consistent_log init_map l}) (i:seq_index l):
+  Lemma (ensures (let lk = to_logk init_map l in
+                  let l' = prefix l i in
+                  lemma_consistent_log_prefix_consistent init_map l i;
+                  let ssm' = to_slot_state_map init_map l' in
+                  lemma_all_entries_valid init_map l i;
+                  index lk i = to_logK_entry ssm' (index l i)))                  
