intermediate/Veritas.Intermediate.Thread.fsti
@@ -1,0 +1,9 @@
+module Veritas.Intermediate.Thread
+
+open Veritas.Intermediate.Logs
+open Veritas.Intermediate.VerifierConfig
+open Veritas.Intermediate.Store
+
+open Veritas.MultiSetHashDomain
+
+let thread_id_logS vcfg = thread_id & logS vcfg
